update Lean

GMLInit/Data/HVal.lean
@@ -1,25 +1,32 @@
 import GMLInit.Data.Basic
 
-inductive HVal.{u} : Type u
-| mk {α : Sort u} : α → HVal
+-- inductive HVal.{u} : Type u
+-- | mk {α : Sort u} : α → HVal
 
-protected def HVal.sort : HVal → Type _
-| @mk α _ => α
+-- protected def HVal.sort : HVal → Type _
+-- | @mk α _ => α
 
-protected def HVal.val : (a : HVal) → a.sort
-| mk a => a
+-- protected def HVal.val : (a : HVal) → a.sort
+-- | @mk _ a => a
+
+structure HVal.{u} where intro ::
+  protected toSort : Sort u
+  protected val : toSort
+
+@[matchPattern]
+def HVal.mk {α} (a : α) : HVal := ⟨α, a⟩
 
 theorem HVal.eq_of_val_heq_val : {a b : HVal} → a.val ≅ b.val → a = b
-| mk _, mk _, HEq.refl _ => Eq.refl _
+| mk _, mk _, HEq.rfl => rfl
 
 theorem HVal.val_heq_val_of_eq : {a b : HVal} → a = b → a.val ≅ b.val
-| mk _, mk _, Eq.refl _ => HEq.refl _
+| mk _, mk _, rfl => HEq.rfl
 
 theorem HVal.eq_iff_val_heq_val (a b : HVal) : a = b ↔ a.val ≅ b.val :=
   ⟨HVal.val_heq_val_of_eq, HVal.eq_of_val_heq_val⟩
 
 theorem HVal.proof_irrel : (a b : HVal.{0}) → a = b
-| @mk a ha, @mk b hb =>
+| ⟨a, ha⟩, ⟨b, hb⟩ =>
   have h : a = b := propext ⟨λ _ => hb, λ _ => ha⟩
   match a, b, h with
   | _, _, rfl => proofIrrel ha hb ▸ rfl
